Update Submission.thy

homework/05/Submission.thy
@@ -4,38 +4,12 @@ begin
 
 inductive ls :: "com \<Rightarrow> state \<Rightarrow> state list \<Rightarrow> state \<Rightarrow> bool" where
   Skip: "ls SKIP s [] s" |
-  Assign: "(v ::= e, s) \<Rightarrow> t \<Longrightarrow> ls (v ::= e) s [] t" |
-  Seq: "\<lbrakk>(c1 ;; c2, s) \<Rightarrow> t; ls c1 s xs t'; ls c2 t' ys t\<rbrakk> \<Longrightarrow> ls (c1 ;; c2) s (xs@t'#ys) t" |
-  IfTrue: "\<lbrakk>bval b s; (c1, s) \<Rightarrow> t; ls c1 s xs t\<rbrakk> \<Longrightarrow> ls (IF b THEN c1 ELSE c2) s (s#xs) t" |
-  IfFalse: "\<lbrakk>\<not>bval b s; (c2, s) \<Rightarrow> t; ls c2 s xs t\<rbrakk> \<Longrightarrow> ls (IF b THEN c1 ELSE c2) s (s#xs) t" |
-  WhileTrue: "\<lbrakk> bval b s1; (c, s1) \<Rightarrow> s2; ls (WHILE b DO c) s2 xs s3 \<rbrakk> \<Longrightarrow> ls (WHILE b DO c) s1 (s1#s2#xs) s3" |
-  WhileFalse: "\<not>bval b s  \<Longrightarrow> ls (WHILE b DO c) s [s] s"
-
-(*
-inductive
-  small_step :: "com * state \<Rightarrow> com * state \<Rightarrow> bool" (infix "\<rightarrow>" 55)
-where
-Assign:  "(x ::= a, s) \<rightarrow> (SKIP, s(x := aval a s))" |
-
-Seq1:    "(SKIP;;c\<^sub>2,s) \<rightarrow> (c\<^sub>2,s)" |
-Seq2:    "(c\<^sub>1,s) \<rightarrow> (c\<^sub>1',s') \<Longrightarrow> (c\<^sub>1;;c\<^sub>2,s) \<rightarrow> (c\<^sub>1';;c\<^sub>2,s')" |
-
-IfTrue:  "bval b s \<Longrightarrow> (IF b THEN c\<^sub>1 ELSE c\<^sub>2,s) \<rightarrow> (c\<^sub>1,s)" |
-IfFalse: "\<not>bval b s \<Longrightarrow> (IF b THEN c\<^sub>1 ELSE c\<^sub>2,s) \<rightarrow> (c\<^sub>2,s)" |
-
-While:   "(WHILE b DO c,s) \<rightarrow>
-            (IF b THEN c;; WHILE b DO c ELSE SKIP,s)"
-*)
-
-(*
-Skip: "ls SKIP s [] s" |
-  Assign: "(v ::= e, s) \<Rightarrow> t \<Longrightarrow> ls (v ::= e) s [] t" |
-  Seq: "\<lbrakk>(c1 ;; c2, s) \<Rightarrow> t; ls c1 s xs t'; ls c2 t' ys t\<rbrakk> \<Longrightarrow> ls (c1 ;; c2) s (xs@t'#ys) t" |
-  IfTrue: "\<lbrakk>bval b s; (IF b THEN c1 ELSE c2, s) \<Rightarrow> t; ls c1 s xs t\<rbrakk> \<Longrightarrow> ls (IF b THEN c1 ELSE c2) s xs t" |
-  IfFalse: "\<lbrakk>\<not>bval b s; (IF b THEN c1 ELSE c2, s) \<Rightarrow> t; ls c2 s xs t\<rbrakk> \<Longrightarrow> ls (IF b THEN c1 ELSE c2) s xs t" |
-  WhileTrue: "\<lbrakk> bval b s1; (c, s1) \<Rightarrow> s2; ls (WHILE b DO c) s2 xs s3 \<rbrakk> \<Longrightarrow> ls (WHILE b DO c) s1 (s2#xs) s3" |
-  WhileFalse: "\<not>bval b s  \<Longrightarrow> ls (WHILE b DO c) s [] s"
-*)
+  Assign: "ls (v ::= e) s [s(v := aval e s)] (s(v := aval e s))" |
+  Seq: "\<lbrakk>ls c1 s xs t'; ls c2 t' ys t\<rbrakk> \<Longrightarrow> ls (c1 ;; c2) s (xs@t'#ys) t" |
+  IfTrue: "\<lbrakk>bval b s; ls c1 s xs t\<rbrakk> \<Longrightarrow> ls (IF b THEN c1 ELSE c2) s (s#xs) t" |
+  IfFalse: "\<lbrakk>\<not>bval b s; ls c2 s xs t\<rbrakk> \<Longrightarrow> ls (IF b THEN c1 ELSE c2) s (s#xs) t" |
+  WhileTrue: "\<lbrakk>bval b s1; ls c s1 xs s2 ; ls (WHILE b DO c) s2 ys s3\<rbrakk> \<Longrightarrow> ls (WHILE b DO c) s1 (s1#s1#xs@s2#ys) s3" |
+  WhileFalse: "\<not>bval b s \<Longrightarrow> ls (WHILE b DO c) s [s, s] s"
 
 declare ls.intros[intro]
 declare ls.cases[elim]
@@ -48,27 +22,106 @@ proof(induction c s t rule: big_step_induct)
 qed auto
 
 theorem ls_big: "ls c s ss t \<Longrightarrow> (c,s) \<Rightarrow> t"
-  by(induction c s ss t rule: ls.induct, auto)
-
-value " ls (SKIP) <> [] <> "
+  by(induction c s ss t rule: ls.induct, blast+)
 
 abbreviation "ss_x c s \<equiv> {map (\<lambda>s. s ''x'') ss |ss t . ls c s ss t}"
 values "ss_x (IF Bc True THEN ''x'' ::= N 3 ELSE ''x'' ::= N 1) <>" \<comment>\<open>[0, 3]\<close>
 values "ss_x (WHILE Less (V ''x'') (N 1) DO ''x'' ::= Plus (V ''x'') (N 1)) <>" \<comment>\<open>[0, 0, 1, 1, 1, 1]\<close>
 
-(*mycases*)
-values "ss_x ( ''x'' ::= N 3;; ''x'' ::= N 4) <>"
-
 lemma ls_step: "\<lbrakk>ls c s ss t; c \<noteq> SKIP\<rbrakk> \<Longrightarrow> (case ss of 
   [] \<Rightarrow> (c,s) \<rightarrow> (SKIP,t) 
 | (x#_) \<Rightarrow> \<exists>c'. (c,s) \<rightarrow> (c',x))"
-  nitpick
-  sorry
+proof(induction c s ss t rule: ls.induct)
+  case (Seq c1 s xs t' c2 ys t)
+  then show ?case
+  proof(cases "xs = Nil")
+    case True
+    then show ?thesis
+      using Seq.hyps(1) by auto
+  next
+    case False
+    then have c1_not_SKIP: "c1 \<noteq> SKIP"
+      using Seq.hyps(1) by auto
+    from False obtain z zs where zzs_def: "xs = z#zs"
+      using list.exhaust_sel by auto
+    with c1_not_SKIP  have "\<exists>c'. (c1, s) \<rightarrow> (c', z)"
+      using Seq.IH(1) by auto
+    then show ?thesis
+      using zzs_def by auto
+  qed
+next
+qed auto
 
 lemma ls_ls: "\<lbrakk>ls c s\<^sub>1 (s\<^sub>2#ss) s\<^sub>3; (c,s\<^sub>1) \<rightarrow> (c',s\<^sub>2)\<rbrakk> \<Longrightarrow> ls c' s\<^sub>2 ss s\<^sub>3"
-  sorry
+proof(induction c s\<^sub>1 "(s\<^sub>2#ss)" s\<^sub>3 arbitrary: ss c' s\<^sub>2 rule: ls.induct)
+  case (Seq c1 s xs t' c2 ys t)
+  then show ?case
+  proof(cases "xs = Nil")
+    case True
+    then have c1_is_SKIP: "c1 = SKIP"
+      using Seq.hyps(1) by auto
+    then have "(c1;;c2,s) \<rightarrow> (c2,s)"
+      by simp
+    then have "c' = c2"
+      using Seq.prems deterministic by blast
+    then show ?thesis
+      using Seq.hyps(3) Seq.hyps(5) True by fastforce
+  next
+    case False
+    then have c1_not_SKIP: "c1 \<noteq> SKIP"
+      using Seq.hyps(1) by auto
+    then obtain c1' where c1_step: "(c1, s) \<rightarrow> (c1', s\<^sub>2)"
+      using Seq.prems by auto
+    have step: "(c1;;c2 ,s) \<rightarrow> (c1';;c2 ,s\<^sub>2)"
+      by (simp add: c1_step)
+    from False obtain z zs where zzs_def: "xs = z#zs"
+      using list.exhaust_sel by auto
+    then have "ls c1' s\<^sub>2 zs t'"
+      using c1_step Seq.hyps(2) Seq.hyps(5) by force
+    then have "ls (c1';;c2) s\<^sub>2 (zs@t'#ys) t"
+      by (simp add: Seq.hyps(3) ls.Seq)
+    moreover
+    have "c' = (c1';;c2)"
+      using Seq.prems deterministic step by fastforce
+    ultimately show ?thesis
+      using Seq.hyps(5) zzs_def by fastforce
+  qed
+next
+  case (WhileTrue b c xs s2 ys s3)
+  then show ?case
+    using ls.IfTrue ls.Seq by fastforce
+qed auto
+
+lemma interstate_not_SKIP: "ls c s (x#xs) t \<Longrightarrow> c \<noteq> SKIP"
+  by(induction c s "(x#xs)" t rule: ls.induct, auto)
 
 theorem ls_steps: "ls c s\<^sub>1 (ss\<^sub>1@[s\<^sub>2]@ss\<^sub>2) t \<Longrightarrow> \<exists>c'. (c,s\<^sub>1) \<rightarrow>* (c',s\<^sub>2)"
-  sorry
+proof(induction ss\<^sub>1 arbitrary: s\<^sub>1 c)
+  case Nil
+  then have ls_simp: "ls c s\<^sub>1 ([s\<^sub>2]@ss\<^sub>2) t"
+    by simp
+  moreover
+  from ls_simp have "c \<noteq> SKIP"
+    by (simp add: interstate_not_SKIP)
+  ultimately have "\<exists>c'. (c,s\<^sub>1) \<rightarrow> (c',s\<^sub>2)"
+    using ls_step by fastforce
+  then show ?case
+    by blast
+next
+  case (Cons a ss\<^sub>1)
+  then have "c \<noteq> SKIP"
+    by (simp add: interstate_not_SKIP)
+  have first_step_ex: "\<exists>c'. (c,s\<^sub>1) \<rightarrow> (c',a)"
+    using Cons.prems ls_step by fastforce
+  then obtain c' where first_step: "(c,s\<^sub>1) \<rightarrow> (c',a)"
+    by blast
+  then have "ls c' a (ss\<^sub>1 @ [s\<^sub>2] @ ss\<^sub>2) t"
+    using Cons.prems ls_ls
+    by simp
+  then have "\<exists>c''. (c', a) \<rightarrow>* (c'', s\<^sub>2)"
+    by (simp add: Cons.IH)
+  then show ?case
+    using first_step star.step by meson
+qed
 
 end
